theories/logrel/term_typing_rules.v
@@ -509,7 +509,7 @@ Section properties.
       { by apply lookup_insert. }
       rewrite Hxc.
       iAssert (c ↣ <? (Xs : ltys Σ kt) (v : val)>
-        MSG v {{ ▷ ltty_car (ktele_app A Xs) v }}; lsty_car (ktele_app S Xs)) with "[Hc]" as "Hc".
+        MSG v {{ ltty_car (ktele_app A Xs) v }}; lsty_car (ktele_app S Xs)) with "[Hc]" as "Hc".
       { iApply (iProto_mapsto_le with "Hc"); iIntros "!>". rewrite HM.
         iApply iProto_le_lmsg_texist. }
       wp_recv (Xs v) as "HA". wp_pures.
